

Lesson 6

METHOD OF SEPARATION OF VARIABLES

In this method, it is assumed that a solution can be expressed as a product or a sum of unknown functions each of which depends on only one of the independent variables.

The success of the method depends on being able to write the resulting eqn so that one side depends only on one variable while the other side depends on the remaining variable so that each side must be a constant.

By repetition of this, the unknown functions can be determined.

The main idea is to convert the given pde into several ode's and then obtain solution by familiar techniques eg

- separation of variables
- homogeneous equations
- exact eqns
- linear eqns etc

This method is the most powerful method of a wide class of pdes where boundary conditions are given i.e. Boundary value problem (BVP)

Given pde of the form

$$Pp + Qq = R \quad \dots (i)$$

or

$$a \frac{\partial u}{\partial x} + b \frac{\partial u}{\partial y} + cu = 0 \quad \dots (ii)$$

Soln:

$$\frac{\partial z}{\partial x} = p, \quad \frac{\partial z}{\partial y} = q$$

$$Z(x, y) \quad \text{or} \quad \psi(x, y)$$

Let the soln be $u(x,y)$

(i) Using a product
 $u(x,y) = X(x) \cdot Y(y)$ --- (i)

The method of soln is to substitute eqn (ii) into eqn 1 and proceed to solve separately for x and y

(ii) Using sum

$$\text{let } u(x,y) = X(x) + Y(y)$$

Given boundary conditions are to be used to obtain a particular solution

Using separable product

$$u(x,y) = X(x) Y(y)$$

$$\frac{du}{dx} = X'Y$$

$$\frac{du}{dy} = XY'$$

Example

Solve the boundary value problem

$$\frac{\partial u}{\partial x} = A \frac{\partial u}{\partial y} \quad u(0,y) = 8e^{-3y}$$

Using method of separation of variables
Soln:

$$\frac{\partial u}{\partial x} = A \frac{\partial u}{\partial y} \quad \text{--- (1)}$$

$$\text{let } u(x,y) = X(x) \cdot Y(y) \quad \text{--- (2)}$$

$$\frac{\partial u}{\partial x} = X'Y, \quad \frac{\partial u}{\partial y} = XY' \quad \text{--- (3)}$$

substitute in original eqn

$$X'Y = AXY'$$

$$\frac{X'}{AX} = \frac{Y'}{Y} = C$$

2 ODEs

$$\frac{y'}{4x} = c$$

and $y' = c$

Recall $\int \frac{f'(x)}{f(x)} = \ln f(x)$

Using logs

$$\frac{1}{4} \int \frac{y'}{x} = \int c$$

$$\Rightarrow \frac{1}{4} \ln x = cx + A$$

$$\frac{1}{4} \log x = cx + \log A$$

$$\log x = 4cx + \log A$$

$$\ln x = 4cx + A$$

$$\log x = 4cx \log e + \log A$$

$$x = A e^{4cx}$$

$$x = A e^{Bx} \quad \dots \quad (4)$$

$$\ln y = cy + D$$

$$y = D e^{cy} \quad \dots \quad (5)$$

Recall $u(x,y) = X(x) \cdot Y(y)$

substitute (4) and (5) into 2

$$u(x,y) = A e^{Bx} \cdot D e^{cy}$$

Let $A \cdot D = M$

$$u(x,y) = M e^{(Bx+cy)}$$

But $B = 4C$

$$u(x,y) = M e^{c(4x+y)}$$

$$u(0,y) = 8 e^{-3y}$$

$$u(0,y) = M e^{c(4x+y)} = M e^{cy}$$

$$= 8 e^{-3y}$$

$$\therefore M = 8 \quad c = -3$$

Particular soln is

$$u(x,y) = 8 e^{-3(4x+y)}$$

Summary

$$\frac{\partial u}{\partial x} = 4 \frac{\partial u}{\partial y}$$

$$p = 4q$$

2) Solve the Initial Value Problem

$$u_x + 2u_y = 0 \quad u(0, y) = (e^{-2y}) \cdot 4$$

Soln

$$\frac{\partial u}{\partial x} + 2 \frac{\partial u}{\partial y} = 0$$

$$u(x, y) = X(x) \cdot Y(y)$$

$$u_x = X'Y \quad u_y = XY'$$

substitute

$$X'Y + 2XY' = 0$$

$$X'Y = -2XY'$$

$$\frac{X'}{2X} = \frac{-Y'}{Y} = k$$

$$2X \quad Y$$

$$\Rightarrow \frac{X'}{2X} = k$$

$$\int \frac{1}{2} \ln X = kx + A$$

$$X = B e^{2kx}$$

$$\Rightarrow \frac{X'}{X} = k = \frac{Y'}{Y} = -k$$

$$\ln Y = -ky + C$$

$$Y = e^{-ky+C}$$

$$Y = e^{-ky} \cdot e^C$$

$$Y = D e^{-ky}$$

$$u(x, y) = X(x) Y(y)$$

$$B e^{2kx} \cdot D e^{-ky}$$

$$= E e^{k(2x-y)}$$

$$u(0, y) = E e^{k(0-y)}$$

$$= E e^{k(-y)}$$

$$4 e^{-2y} = E e^{-ky}$$

$$E = 4; \quad k = (-2) \Rightarrow 2$$

Particular soln

$$u(x, y) = 4 e^{-2(2x-y)}$$

$$= 4 e^{4x-2y}$$

Exercise

$$1. \frac{\partial u}{\partial x} - x \frac{\partial u}{\partial y} = 0$$

$$2. 3u_x + 2u_y = 0$$

$$u(x, 0) = Ae^{-x}$$

$$3. u_x + u = u_y$$

$$u(x, 0) = Ae^{-3x}$$

$$4. Au_x + u_y = 3u$$

$$u = 3e^{-y} - e^{5y} \quad \text{where } x = 0$$